\begin{answer}

\begin{eqnarray*}
p(t^{(i)}=1\mid y^{(i)} = 1, x^{(i)}) 
&=& \frac{p(y^{(i)}=1\mid t^{(i)} = 1, x^{(i)})p(t^{(i)}=1\mid x^{(i)}) }{p(y^{(i)}=1\mid x^{(i)})}\\
&=& \frac{p(y^{(i)}=1\mid t^{(i)} = 1, x^{(i)})p(t^{(i)}=1\mid x^{(i)})}{p(y^{(i)}=1\mid t^{(i)} = 1, x^{(i)})p(t^{(i)}=1\mid x^{(i)}) +p(y^{(i)}=1\mid t^{(i)} = 0, x^{(i)})p(t^{(i)}=0\mid x^{(i)}) }\\
&=& \frac{p(y^{(i)}=1\mid t^{(i)} = 1, x^{(i)})p(t^{(i)}=1\mid x^{(i)})}{p(y^{(i)}=1\mid t^{(i)} = 1, x^{(i)})p(t^{(i)}=1\mid x^{(i)}) +0p(t^{(i)}=0\mid x^{(i)}) }\\
&=& \frac{p(y^{(i)}=1\mid t^{(i)} = 1, x^{(i)})p(t^{(i)}=1\mid x^{(i)})}{p(y^{(i)}=1\mid t^{(i)} = 1, x^{(i)})p(t^{(i)}=1\mid x^{(i)})}\\
&=& 1

\end{eqnarray*}
\end{answer}
