\begin{answer}

From (d) we now that  

\begin{eqnarray*}
 h(x^{(i)}) &=& p(y^{(i)} = 1\mid x^{(i)}) \\
 &=&\alpha p(t^{(i)} = 1\mid x^{(i)})\\
\end{eqnarray*}
 
Assuming $g(x^{(i)}) =p(t^{(i)} = 1\mid x^{(i)})$, we have that
 
\begin{eqnarray*}
\mathbb{E}[h(x^{(i)})\mid y^{(i)}=1]  &=&
\mathbb{E}[\alpha g(x^{(i)})\mid y^{(i)}=1 ] \\
&=& \alpha \mathbb{E}[g(x^{(i)})\mid y^{(i)}=1 ] \\
&=& \alpha \mathbb{E}[p(t^{(i)} = 1\mid x^{(i)})\mid y^{(i)}=1 ] 
\end{eqnarray*}

From (c) we now that $p(t^{(i)}=1\mid y^{(i)} = 1, x^{(i)}) = 1$ then $\mathbb{E}[p(t^{(i)} = 1\mid x^{(i)})\mid y^{(i)}=1 ] = 1$
Therefore $\mathbb{E}[h(x^{(i)})\mid y^{(i)}=1] = \alpha$
\end{answer}
