\begin{answer}
The posterior distribution can be written base on Bayer Rules: 
%
\begin{eqnarray*}
	p(y = 1\mid x; \phi, \mu_0, \mu_1, \Sigma) &=& \frac{p(x\mid y=1; \phi, \mu_0, \mu_1, \Sigma) p(y = 1; \phi, \mu_0, \mu_1, \Sigma)}{p(x; \phi, \mu_0, \mu_1, \Sigma)} \\
&=& \frac{\exp\left(-\frac{1}{2}(x-\mu_1)^T \Sigma^{-1} (x-\mu_1) \right)\phi}{\exp\left(-\frac{1}{2}(x-\mu_1)^T \Sigma^{-1} (x-\mu_1) \right)\phi +\exp\left(-\frac{1}{2}(x-\mu_{0})^T \Sigma^{-1} (x-\mu_{0})\right) (1-\phi) }\\
&=& \frac{1}{1+ \frac{ 1- \theta}{\theta} \exp\left(-\frac{1}{2}(x-\mu_{0})^T \Sigma^{-1} (x-\mu_{0}) + \frac{1}{2}(x-\mu_1)^T \Sigma^{-1} (x-\mu_1) \right) }\\
&=& \frac{1}{1+  \exp\left(\log(\frac{ 1- \theta}{\theta})-\frac{1}{2}(x-\mu_{0})^T \Sigma^{-1} (x-\mu_{0}) + \frac{1}{2}(x-\mu_1)^T \Sigma^{-1} (x-\mu_1) \right) }\\
&=& \frac{1}{1+  \exp\left(\log(\frac{ 1- \theta}{\theta})+\frac{1}{2} [- A + B ] \right) }
\end{eqnarray*}

where  $A = (x-\mu_{0})^T \Sigma^{-1} (x-\mu_{0})$ and  $B = (x-\mu_1)^T \Sigma^{-1} (x-\mu_1)$. We can expand the difference $-A + B$:

\begin{eqnarray*}
B-A &=& (x-\mu_{1}^T)\Sigma^{-1} (x-\mu_{1}) - (x-\mu_{0})^T \Sigma^{-1} (x-\mu_{0})\\
&=& x^T\Sigma^{-1}x -x^T\Sigma^{-1}\mu_{1} -\mu_{1}^T\Sigma^{-1}x + \mu_{1}^T\Sigma^{-1}\mu_{1} -x^T\Sigma^{-1}x +x^T\Sigma^{-1}\mu_{0} +\mu_{0}^T\Sigma^{-1}x -\mu_{0}^T\Sigma^{-1}\mu_{0} \\
&=& -2\mu_{1}^T\Sigma^{-1}x + \mu_{1}^T\Sigma^{-1}\mu_{1} +2\mu_{0}^T\Sigma^{-1}x -\mu_{0}^T\Sigma^{-1}\mu_{0} \\
&=& 2(\mu_{0} - \mu_{1})^T\Sigma^{-1}x + \mu_{1}^T\Sigma^{-1}\mu_{1} -\mu_{0}^T\Sigma^{-1}\mu_{0}
\end{eqnarray*}

then we have:
\begin{eqnarray*}
p(y = 1\mid x; \phi, \mu_0, \mu_1, \Sigma) &=& \frac{1}{1+  \exp\left(\log(\frac{ 1- \theta}{\theta})+ (\mu_{0} - \mu_{1})^T\Sigma^{-1}x + \frac{1}{2}\mu_{1}^T\Sigma^{-1}\mu_{1} -\frac{1}{2}\mu_{0}^T\Sigma^{-1}\mu_{0} \right) }
\end{eqnarray*}

Taking $\theta^T = -(\mu_{0} - \mu_{1})^T\Sigma^{-1}$ and $\theta_{0} =-\log(\frac{ 1- \theta}{\theta})-  \frac{1}{2}\mu_{1}^T\Sigma^{-1}\mu_{1} +\frac{1}{2}\mu_{0}^T\Sigma^{-1}\mu_{0}$ 

obtain that

\begin{eqnarray*}
p(y = 1\mid x; \phi, \mu_0, \mu_1, \Sigma) &=& \frac{1}{1+  \exp\left( -(\theta^{T}x + \theta_{0}) \right) }
\end{eqnarray*}


%

\end{answer}
