\begin{answer}

Solution 1 : 
The exponential family have the form 
\begin{equation*}
    p(y ; \eta) = b(y)\exp(\eta y - a(\eta)).
\end{equation*}

because $p(y ; \eta)$ is a probability family distribution, we have: 

\begin{equation*}
\int p(y ; \eta) dy = \int b(y)\exp(\eta y - a(\eta)) dy = 1
\end{equation*}

which implies
\begin{equation*}
    a(\eta) = \log \int b(y)\exp(\eta y) dy
\end{equation*}

then the first derivative of $a(\eta)$ is 

\begin{align*}
    \frac{\partial}{\partial \eta} a(\eta)  &= \frac{\partial}{\partial \eta} \log \int b(y)\exp(\eta y)dy && \text{}\\
     &=\frac{\int b(y)\exp(\eta y) y dy}{ \int b(y)\exp(\eta y) dy}  && \text{}\\
     &=\frac{\int b(y)\exp(\eta y) ydy}{\exp(a(\eta))} \\ 
     &= \int b(y)\exp(\eta y - a(\eta))y dy \\
     &= \int  p(y ; \eta)y dy \\
     &= \mathbb{E}[Y ;\eta] 
\end{align*}

\end{answer}
